src/examples/Kuiper.ArrayView.Test.EvenOdds3.fst
@@ -21,12 +21,16 @@ let strided_view et (len : nat) (stride : nat) (offset : natlt stride) :
   aview et len (lseq et ((len + stride - 1 - offset) / stride))
 = {
   iview = {
-    ait = natlt ((len + stride - 1 - offset) / stride);
-    ait_enum = solve;
-    imap = {
-      f = (fun (i : natlt ((len + stride - 1 - offset) / stride)) -> i * stride + offset <: natlt len);
-      is_inj = ez;
-    }
+    sch = {
+      ait = natlt ((len + stride - 1 - offset) / stride);
+      ait_enum = solve;
+    };
+    step = {
+      imap = {
+        f = (fun (i : natlt ((len + stride - 1 - offset) / stride)) -> i * stride + offset <: natlt len);
+        is_inj = ez;
+      };
+    };
   };
   igm = solve;
 }
@@ -41,13 +45,17 @@ instance _cview_strided
 : IView.ciview (strided_view et len stride offset).iview
 = {
   fits = ez;
-  cit  = szlt ((len + stride - 1 - offset) / stride);
-  bij  = natural;
-  imap = {
-    f = (fun (i : szlt ((len + stride - 1 - offset) / stride)) -> i `SZ.mul` stride `SZ.add` offset <: szlt len);
-    is_inj = ez;
+  sch = {
+    cit  = szlt ((len + stride - 1 - offset) / stride);
+    bij  = natural;
   };
-  compat = ez;
+  step = {
+    cimap = {
+      f = (fun (i : szlt ((len + stride - 1 - offset) / stride)) -> i `SZ.mul` stride `SZ.add` offset <: szlt len);
+      is_inj = ez;
+    };
+    compat = ez;
+  };
 }
 
 inline_for_extraction noextract
@@ -61,14 +69,14 @@ instance _cview_odd #et (#len : erased nat{SZ.fits len}) : IView.ciview (odd_vie
 (* What is happening?!?! Why isn't this obvious? *)
 
 let _wat_even (#len : nat{SZ.fits len}) :
-  Lemma (reveal (_cview_even #u32 #len).bij == fin_size_t_bij ((len + 2 - 1 - 0) / 2))
+  Lemma (reveal (_cview_even #u32 #len).sch.bij == fin_size_t_bij ((len + 2 - 1 - 0) / 2))
         [SMTPat (_cview_even #u32 #len)]
-= assert_norm (reveal (_cview_even #u32 #len).bij == fin_size_t_bij ((len + 2 - 1 - 0) / 2))
+= assert_norm (reveal (_cview_even #u32 #len).sch.bij == fin_size_t_bij ((len + 2 - 1 - 0) / 2))
 
 let _wat_odd (#len : nat{SZ.fits len}) :
-  Lemma (reveal (_cview_odd #u32 #len).bij == fin_size_t_bij ((len + 2 - 1 - 1) / 2))
+  Lemma (reveal (_cview_odd #u32 #len).sch.bij == fin_size_t_bij ((len + 2 - 1 - 1) / 2))
         [SMTPat (_cview_odd #u32 #len)]
-= assert_norm (reveal (_cview_odd #u32 #len).bij == fin_size_t_bij ((len + 2 - 1 - 1) / 2))
+= () // assert_norm (reveal (_cview_odd #u32 #len).bij == fin_size_t_bij ((len + 2 - 1 - 1) / 2))
 
 let _sanity1 (#len : nat{SZ.fits len}) (x : szlt ((len + 1) / 2)) : Lemma (ci_to_ai (even_view u32 len) x == SZ.v x)
   = ()
@@ -143,8 +151,8 @@ let it_of_nat_lem (#len:nat) (i : natlt len)
   = ()
 
 let all_in_image (len:nat) (i : nat)
-  : Lemma (i < len ==> in_image (sum_aview (even_view u32 len) (odd_view u32 len)).iview.imap.f i)
-          [SMTPat (in_image (sum_aview (even_view u32 len) (odd_view u32 len)).iview.imap.f i)]
+  : Lemma (i < len ==> in_image (sum_aview (even_view u32 len) (odd_view u32 len)).iview.step.imap.f i)
+          [SMTPat (in_image (sum_aview (even_view u32 len) (odd_view u32 len)).iview.step.imap.f i)]
   = if i < len then (let j = __it_of_nat #len i in it_of_nat_lem #len i)
 
 let merge_lemma #et (#len:nat) (sl : lseq et ((len + 1) / 2)) (sr : lseq et (len / 2))
@@ -180,36 +188,39 @@ let split_lemma #et (#len:nat) (s : lseq et len)
             (to_seq (sum_aview (even_view et len) (odd_view et len)) (seq_evens s, seq_odds s))
             s)
 
+#push-options "--z3rlimit 20"
 fn test_write (a : gpu_array u32 100)
     (#v0 : erased (lseq u32 100))
     preserves gpu
     requires a |-> v0
     ensures  a |-> Seq.upd (Seq.upd v0 20 42ul) 41 43ul
-  {
-    varray_abs' vw a;
-    let va = from_array vw a;
+{
+  varray_abs' vw a;
+  let va = from_array vw a;
 
-    let vl, vr = varray_split2
-      (even_view u32 100)
-      (odd_view u32 100)
-      (from_array vw a)
-      #_
-      #(from_seq vw v0) // ARGH, why do I have to provide this!?!??! terrible error otherwise
-      ;
-    // Note: that doesn't happen if we use split2_, the ghost version
+  let vl, vr = varray_split2
+    (even_view u32 100)
+    (odd_view u32 100)
+    (from_array vw a)
+    #_
+    #(from_seq vw v0) // ARGH, why do I have to provide this!?!??! terrible error otherwise
+    ;
+  // Note: that doesn't happen if we use split2_, the ghost version
 
-    varray_write vl 10sz 42ul;
-    varray_write vr 20sz 43ul;
+  varray_write vl 10sz 42ul;
+  varray_write vr 20sz 43ul;
 
-    let va = varray_join2 vl vr;
+  let va = varray_join2 vl vr;
 
-    varray_concr va;
+  varray_concr va;
 
-    rewrite each core va as a;
+  rewrite each core va as a;
 
-    with v1.
-      assert (a |-> v1);
-      assert (pure (Seq.equal v1 (Seq.upd (Seq.upd v0 20 42ul) 41 43ul))); // use extensionality
+  with v1.
+    assert (a |-> v1);
+    // assert (pure (Seq.equal v1 (Seq.upd v0 20 42ul)));
+    assert (pure (Seq.equal v1 (Seq.upd (Seq.upd v0 20 42ul) 41 43ul))); // use extensionality
 
-    ()
-  }
+  ()
+}
+#pop-options
