src/lib/views/Kuiper.IView.fst
@@ -5,6 +5,6 @@ module Kuiper.IView
 let full_iff_cardinal
   (#len : nat)
   (vw : aiview len)
-  : Lemma (is_full_view vw <==> vw.ait_enum._cardinal == len)
+  : Lemma (is_full_view vw <==> vw.sch.ait_enum._cardinal == len)
           [SMTPat (is_full_view vw)]
   = admit()
